<?xml version="1.0"?>
<rdf:RDF xmlns="http://emmc.info/emmo-material#"
     xml:base="http://emmc.info/emmo-material"
     xmlns:owl="http://www.w3.org/2002/07/owl#"
     xmlns:rdf="http://www.w3.org/1999/02/22-rdf-syntax-ns#"
     xmlns:xml="http://www.w3.org/XML/1998/namespace"
     xmlns:xsd="http://www.w3.org/2001/XMLSchema#"
     xmlns:rdfs="http://www.w3.org/2000/01/rdf-schema#"
     xmlns:emmo-core="http://emmc.info/emmo-core#"
     xmlns:emmo-direct="http://emmc.info/emmo-direct#"
     xmlns:emmo-material="http://emmc.info/emmo-material#">
    <owl:Ontology rdf:about="http://emmc.info/emmo-material">
        <owl:imports rdf:resource="http://emmc.info/emmo-direct"/>
    </owl:Ontology>



    <!--
    ///////////////////////////////////////////////////////////////////////////////////////
    //
    // Classes
    //
    ///////////////////////////////////////////////////////////////////////////////////////
     -->




    <!-- http://emmc.info/emmo-core#EMMO_0f795e3e_c602_4577_9a43_d5a231aa1360 -->

    <rdf:Description rdf:about="http://emmc.info/emmo-core#EMMO_0f795e3e_c602_4577_9a43_d5a231aa1360">
        <owl:disjointUnionOf rdf:parseType="Collection">
            <rdf:Description rdf:about="http://emmc.info/emmo-material#EMMO_385b8f6e_43ac_4596_ad76_ac322c68b7ca"/>
            <rdf:Description rdf:about="http://emmc.info/emmo-material#EMMO_e5488299_8dab_4ebb_900a_26d2abed8396"/>
        </owl:disjointUnionOf>
    </rdf:Description>



    <!-- http://emmc.info/emmo-material#EMMO_1067b97a_84f8_4d22_8ace_b842b8ce355c -->

    <owl:Class rdf:about="http://emmc.info/emmo-material#EMMO_1067b97a_84f8_4d22_8ace_b842b8ce355c">
        <rdfs:subClassOf rdf:resource="http://emmc.info/emmo-material#EMMO_7d66bde4_b68d_41cc_b5fc_6fd98c5e2ff0"/>
        <rdfs:subClassOf>
            <owl:Restriction>
                <owl:onProperty rdf:resource="http://emmc.info/emmo-direct#EMMO_b2282816_b7a3_44c6_b2cb_3feff1ceb7fe"/>
                <owl:someValuesFrom rdf:resource="http://emmc.info/emmo-material#EMMO_8043d3c6_a4c1_4089_ba34_9744e28e5b3d"/>
            </owl:Restriction>
        </rdfs:subClassOf>
        <emmo-core:EMMO_967080e5_2f42_4eb2_a3a9_c58143e835f9>A &apos;spacetime&apos; that stands for a quantum system made of electrons.</emmo-core:EMMO_967080e5_2f42_4eb2_a3a9_c58143e835f9>
        <rdfs:label xml:lang="en">electron_cloud</rdfs:label>
    </owl:Class>



    <!-- http://emmc.info/emmo-material#EMMO_174cf221_9d16_427c_abea_e217a948969b -->

    <owl:Class rdf:about="http://emmc.info/emmo-material#EMMO_174cf221_9d16_427c_abea_e217a948969b">
        <rdfs:subClassOf rdf:resource="http://emmc.info/emmo-direct#EMMO_36c79456_e29c_400d_8bd3_0eedddb82652"/>
        <rdfs:label xml:lang="en">mesoscopic</rdfs:label>
    </owl:Class>



    <!-- http://emmc.info/emmo-material#EMMO_25f8b804_9a0b_4387_a3e7_b35bce5365ee -->

    <owl:Class rdf:about="http://emmc.info/emmo-material#EMMO_25f8b804_9a0b_4387_a3e7_b35bce5365ee">
        <rdfs:label xml:lang="en">photon</rdfs:label>
    </owl:Class>



    <!-- http://emmc.info/emmo-material#EMMO_2fd3f574_5e93_47fe_afca_ed80b0a21ab4 -->

    <owl:Class rdf:about="http://emmc.info/emmo-material#EMMO_2fd3f574_5e93_47fe_afca_ed80b0a21ab4">
        <rdfs:subClassOf rdf:resource="http://emmc.info/emmo-material#EMMO_eb77076b_a104_42ac_a065_798b2d2809ad"/>
        <owl:disjointUnionOf rdf:parseType="Collection">
            <rdf:Description rdf:about="http://emmc.info/emmo-material#EMMO_4588526f_8553_4f4d_aa73_a483e88d599b"/>
            <rdf:Description rdf:about="http://emmc.info/emmo-material#EMMO_db03061b_db31_4132_a47a_6a634846578b"/>
        </owl:disjointUnionOf>
        <emmo-core:EMMO_967080e5_2f42_4eb2_a3a9_c58143e835f9>An atom that does not share electrons with other atoms.</emmo-core:EMMO_967080e5_2f42_4eb2_a3a9_c58143e835f9>
        <rdfs:comment>A standalone atom can be bonded with other atoms by intermolecular forces (i.e. dipole–dipole, London dispersion force, hydrogen bonding), since this bonds does not involve electron sharing.</rdfs:comment>
        <rdfs:label xml:lang="en">standalone_atom</rdfs:label>
    </owl:Class>



    <!-- http://emmc.info/emmo-material#EMMO_3397f270_dfc1_4500_8f6f_4d0d85ac5f71 -->

    <owl:Class rdf:about="http://emmc.info/emmo-material#EMMO_3397f270_dfc1_4500_8f6f_4d0d85ac5f71">
        <rdfs:subClassOf rdf:resource="http://emmc.info/emmo-material#EMMO_174cf221_9d16_427c_abea_e217a948969b"/>
        <rdfs:subClassOf>
            <owl:Restriction>
                <owl:onProperty rdf:resource="http://emmc.info/emmo-direct#EMMO_b2282816_b7a3_44c6_b2cb_3feff1ceb7fe"/>
                <owl:minQualifiedCardinality rdf:datatype="http://www.w3.org/2001/XMLSchema#nonNegativeInteger">2</owl:minQualifiedCardinality>
                <owl:onClass rdf:resource="http://emmc.info/emmo-material#EMMO_8303a247_f9d9_4616_bdcd_f5cbd7b298e3"/>
            </owl:Restriction>
        </rdfs:subClassOf>
        <rdfs:subClassOf>
            <owl:Restriction>
                <owl:onProperty rdf:resource="http://emmc.info/emmo-direct#EMMO_b2282816_b7a3_44c6_b2cb_3feff1ceb7fe"/>
                <owl:qualifiedCardinality rdf:datatype="http://www.w3.org/2001/XMLSchema#nonNegativeInteger">1</owl:qualifiedCardinality>
                <owl:onClass rdf:resource="http://emmc.info/emmo-material#EMMO_1067b97a_84f8_4d22_8ace_b842b8ce355c"/>
            </owl:Restriction>
        </rdfs:subClassOf>
        <emmo-core:EMMO_967080e5_2f42_4eb2_a3a9_c58143e835f9>An atom_based state defined by an exact number of e-bonded atomic species and an electron cloud made of the shared electrons.</emmo-core:EMMO_967080e5_2f42_4eb2_a3a9_c58143e835f9>
        <emmo-core:EMMO_b432d2d5_25f4_4165_99c5_5935a7763c1a>H20, C6H12O6, CH4</emmo-core:EMMO_b432d2d5_25f4_4165_99c5_5935a7763c1a>
        <rdfs:comment>An entity is called essential if removing one direct part will lead to a change in entity class.

An entity is called redundand if removing one direct part will not lead to a change in entity class.</rdfs:comment>
        <rdfs:comment>This definition states that this object is a non-periodic set of atoms or a set with a finite periodicity.

Removing an atom from the state will result in another type of atom_based state.

e.g. you cannot remove H from H20 without changing the molecule type (essential). However, you can remove a C from a nanotube (redundant). C60 fullerene is a molecule, since it has a finite periodicity and is made of a well defined number of atoms (essential). A C nanotube is not a molecule, since it has an infinite periodicity (redundant).</rdfs:comment>
        <rdfs:label xml:lang="en">molecule</rdfs:label>
    </owl:Class>



    <!-- http://emmc.info/emmo-material#EMMO_385b8f6e_43ac_4596_ad76_ac322c68b7ca -->

    <owl:Class rdf:about="http://emmc.info/emmo-material#EMMO_385b8f6e_43ac_4596_ad76_ac322c68b7ca">
        <rdfs:subClassOf rdf:resource="http://emmc.info/emmo-core#EMMO_0f795e3e_c602_4577_9a43_d5a231aa1360"/>
        <owl:disjointUnionOf rdf:parseType="Collection">
            <rdf:Description rdf:about="http://emmc.info/emmo-material#EMMO_72d53756_7fb1_46ed_980f_83f47efbe105"/>
            <rdf:Description rdf:about="http://emmc.info/emmo-material#EMMO_8043d3c6_a4c1_4089_ba34_9744e28e5b3d"/>
        </owl:disjointUnionOf>
        <rdfs:label xml:lang="en">massive</rdfs:label>
    </owl:Class>



    <!-- http://emmc.info/emmo-material#EMMO_3c218fbe_60c9_4597_8bcf_41eb1773af1f -->

    <owl:Class rdf:about="http://emmc.info/emmo-material#EMMO_3c218fbe_60c9_4597_8bcf_41eb1773af1f">
        <owl:equivalentClass>
            <owl:Class>
                <owl:intersectionOf rdf:parseType="Collection">
                    <rdf:Description rdf:about="http://emmc.info/emmo-core#EMMO_c5ddfdba_c074_4aa4_ad6b_1ac4942d300d"/>
                    <owl:Class>
                        <owl:complementOf>
                            <owl:Restriction>
                                <owl:onProperty rdf:resource="http://emmc.info/emmo-core#EMMO_17e27c22_37e1_468c_9dd7_95e137f73e7f"/>
                                <owl:someValuesFrom rdf:resource="http://emmc.info/emmo-material#EMMO_385b8f6e_43ac_4596_ad76_ac322c68b7ca"/>
                            </owl:Restriction>
                        </owl:complementOf>
                    </owl:Class>
                </owl:intersectionOf>
            </owl:Class>
        </owl:equivalentClass>
        <rdfs:label xml:lang="en">vacuum</rdfs:label>
    </owl:Class>



    <!-- http://emmc.info/emmo-material#EMMO_4588526f_8553_4f4d_aa73_a483e88d599b -->

    <owl:Class rdf:about="http://emmc.info/emmo-material#EMMO_4588526f_8553_4f4d_aa73_a483e88d599b">
        <emmo-core:EMMO_967080e5_2f42_4eb2_a3a9_c58143e835f9>A standalone atom that has no net charge.</emmo-core:EMMO_967080e5_2f42_4eb2_a3a9_c58143e835f9>
        <rdfs:label xml:lang="en">neutral_atom</rdfs:label>
    </owl:Class>



    <!-- http://emmc.info/emmo-material#EMMO_50781fd9_a9e4_46ad_b7be_4500371d188d -->

    <owl:Class rdf:about="http://emmc.info/emmo-material#EMMO_50781fd9_a9e4_46ad_b7be_4500371d188d">
        <rdfs:subClassOf rdf:resource="http://emmc.info/emmo-material#EMMO_7d66bde4_b68d_41cc_b5fc_6fd98c5e2ff0"/>
        <owl:disjointUnionOf rdf:parseType="Collection">
            <rdf:Description rdf:about="http://emmc.info/emmo-material#EMMO_8f87e700_99a8_4427_8ffb_e493de05c217"/>
            <rdf:Description rdf:about="http://emmc.info/emmo-material#EMMO_df808271_df91_4f27_ba59_fa423c51896c"/>
        </owl:disjointUnionOf>
        <rdfs:label xml:lang="en">nucleon</rdfs:label>
    </owl:Class>



    <!-- http://emmc.info/emmo-material#EMMO_5b2222df_4da6_442f_8244_96e9e45887d1 -->

    <owl:Class rdf:about="http://emmc.info/emmo-material#EMMO_5b2222df_4da6_442f_8244_96e9e45887d1">
        <owl:equivalentClass>
            <owl:Restriction>
                <owl:onProperty rdf:resource="http://emmc.info/emmo-core#EMMO_17e27c22_37e1_468c_9dd7_95e137f73e7f"/>
                <owl:someValuesFrom rdf:resource="http://emmc.info/emmo-material#EMMO_385b8f6e_43ac_4596_ad76_ac322c68b7ca"/>
            </owl:Restriction>
        </owl:equivalentClass>
        <rdfs:subClassOf>
            <owl:Restriction>
                <owl:onProperty rdf:resource="http://emmc.info/emmo-core#EMMO_85fc27bc_5e42_4baa_bf85_5a2dc4a26a1f"/>
                <owl:allValuesFrom rdf:resource="http://emmc.info/emmo-material#EMMO_5b2222df_4da6_442f_8244_96e9e45887d1"/>
            </owl:Restriction>
        </rdfs:subClassOf>
        <rdfs:label xml:lang="en">matter</rdfs:label>
    </owl:Class>



    <!-- http://emmc.info/emmo-material#EMMO_5c4aff3c_c30c_4507_86d5_b4df41eb9f2f -->

    <owl:Class rdf:about="http://emmc.info/emmo-material#EMMO_5c4aff3c_c30c_4507_86d5_b4df41eb9f2f">
        <rdfs:subClassOf rdf:resource="http://emmc.info/emmo-direct#EMMO_36c79456_e29c_400d_8bd3_0eedddb82652"/>
        <rdfs:label xml:lang="en">atomic</rdfs:label>
    </owl:Class>



    <!-- http://emmc.info/emmo-material#EMMO_72d53756_7fb1_46ed_980f_83f47efbe105 -->

    <owl:Class rdf:about="http://emmc.info/emmo-material#EMMO_72d53756_7fb1_46ed_980f_83f47efbe105">
        <rdfs:label xml:lang="en">quark</rdfs:label>
    </owl:Class>



    <!-- http://emmc.info/emmo-material#EMMO_7d66bde4_b68d_41cc_b5fc_6fd98c5e2ff0 -->

    <owl:Class rdf:about="http://emmc.info/emmo-material#EMMO_7d66bde4_b68d_41cc_b5fc_6fd98c5e2ff0">
        <rdfs:subClassOf rdf:resource="http://emmc.info/emmo-direct#EMMO_36c79456_e29c_400d_8bd3_0eedddb82652"/>
        <rdfs:label xml:lang="en">subatomic</rdfs:label>
    </owl:Class>



    <!-- http://emmc.info/emmo-material#EMMO_7db59e56_f68b_48b7_ae99_891c35ae5c3b -->

    <owl:Class rdf:about="http://emmc.info/emmo-material#EMMO_7db59e56_f68b_48b7_ae99_891c35ae5c3b">
        <rdfs:label xml:lang="en">gluon</rdfs:label>
    </owl:Class>



    <!-- http://emmc.info/emmo-material#EMMO_8043d3c6_a4c1_4089_ba34_9744e28e5b3d -->

    <owl:Class rdf:about="http://emmc.info/emmo-material#EMMO_8043d3c6_a4c1_4089_ba34_9744e28e5b3d">
        <rdfs:label xml:lang="en">electron</rdfs:label>
    </owl:Class>



    <!-- http://emmc.info/emmo-material#EMMO_8303a247_f9d9_4616_bdcd_f5cbd7b298e3 -->

    <owl:Class rdf:about="http://emmc.info/emmo-material#EMMO_8303a247_f9d9_4616_bdcd_f5cbd7b298e3">
        <rdfs:subClassOf rdf:resource="http://emmc.info/emmo-material#EMMO_eb77076b_a104_42ac_a065_798b2d2809ad"/>
        <emmo-core:EMMO_967080e5_2f42_4eb2_a3a9_c58143e835f9>An electronic bonded atom that shares at least one electron to the atom_based entity of which is part of.</emmo-core:EMMO_967080e5_2f42_4eb2_a3a9_c58143e835f9>
        <rdfs:comment>A real bond between atoms is always something hybrid between covalent, metallic and ionic.

In general, metallic and ionic bonds have atoms sharing electrons.</rdfs:comment>
        <rdfs:comment>The bond types that are covered by this definition are the strong electonic bonds: covalent, metallic and ionic.</rdfs:comment>
        <rdfs:comment>This class can be used to represent molecules as simplified quantum systems, in which outer molecule shared electrons are un-entangled with the inner shells of the atoms composing the molecule.</rdfs:comment>
        <rdfs:label xml:lang="en">e-bonded_atom</rdfs:label>
    </owl:Class>



    <!-- http://emmc.info/emmo-material#EMMO_87ac88ff_8379_4f5a_8c7b_424a8fff1ee8 -->

    <owl:Class rdf:about="http://emmc.info/emmo-material#EMMO_87ac88ff_8379_4f5a_8c7b_424a8fff1ee8">
        <rdfs:subClassOf rdf:resource="http://emmc.info/emmo-material#EMMO_8b0923ab_b500_477b_9ce9_8b3a3e4dc4f2"/>
        <emmo-core:EMMO_967080e5_2f42_4eb2_a3a9_c58143e835f9>A continuum that has no fixed shape and yields easily to external pressure.</emmo-core:EMMO_967080e5_2f42_4eb2_a3a9_c58143e835f9>
        <emmo-core:EMMO_b432d2d5_25f4_4165_99c5_5935a7763c1a>Gas, liquid, plasma,</emmo-core:EMMO_b432d2d5_25f4_4165_99c5_5935a7763c1a>
        <rdfs:label xml:lang="en">fluid</rdfs:label>
    </owl:Class>



    <!-- http://emmc.info/emmo-material#EMMO_8b0923ab_b500_477b_9ce9_8b3a3e4dc4f2 -->

    <owl:Class rdf:about="http://emmc.info/emmo-material#EMMO_8b0923ab_b500_477b_9ce9_8b3a3e4dc4f2">
        <rdfs:subClassOf rdf:resource="http://emmc.info/emmo-direct#EMMO_36c79456_e29c_400d_8bd3_0eedddb82652"/>
        <emmo-core:EMMO_967080e5_2f42_4eb2_a3a9_c58143e835f9>A state that is a collection of sufficiently large number of other parts such that:
- it is the bearer of qualities that can exists only by the fact that it is a sum of parts
- the smallest partition dV of the state volume in which we are interested in, contains enough parts to be statistically consistent: n [#/m3] x dV [m3] &gt;&gt; 1</emmo-core:EMMO_967080e5_2f42_4eb2_a3a9_c58143e835f9>
        <rdfs:comment>A continuum is made of a sufficient number of parts that it continues to exists as continuum individual even after the loss of one of them i.e. a continuum is a redundant.</rdfs:comment>
        <rdfs:comment>A continuum is not necessarily small (i.e. composed by the minimum amount of sates to fulfill the definition).

A single continuum individual can be the whole fluid in a pipe.</rdfs:comment>
        <rdfs:comment>A continuum is the bearer of properties that are generated by the interactions of parts such as viscosity and thermal or electrical conductivity.</rdfs:comment>
        <rdfs:label xml:lang="en">continuum</rdfs:label>
    </owl:Class>



    <!-- http://emmc.info/emmo-material#EMMO_8f87e700_99a8_4427_8ffb_e493de05c217 -->

    <owl:Class rdf:about="http://emmc.info/emmo-material#EMMO_8f87e700_99a8_4427_8ffb_e493de05c217">
        <rdfs:subClassOf>
            <owl:Restriction>
                <owl:onProperty rdf:resource="http://emmc.info/emmo-direct#EMMO_b2282816_b7a3_44c6_b2cb_3feff1ceb7fe"/>
                <owl:someValuesFrom rdf:resource="http://emmc.info/emmo-material#EMMO_72d53756_7fb1_46ed_980f_83f47efbe105"/>
            </owl:Restriction>
        </rdfs:subClassOf>
        <rdfs:label xml:lang="en">proton</rdfs:label>
    </owl:Class>



    <!-- http://emmc.info/emmo-material#EMMO_a2b006f2_bbfd_4dba_bcaa_3fca20cd6be1 -->

    <owl:Class rdf:about="http://emmc.info/emmo-material#EMMO_a2b006f2_bbfd_4dba_bcaa_3fca20cd6be1">
        <rdfs:subClassOf rdf:resource="http://emmc.info/emmo-material#EMMO_8b0923ab_b500_477b_9ce9_8b3a3e4dc4f2"/>
        <emmo-core:EMMO_967080e5_2f42_4eb2_a3a9_c58143e835f9>A continuum characterized by structural rigidity and resistance to changes of shape or volume, that retains its shape and density when not confined.</emmo-core:EMMO_967080e5_2f42_4eb2_a3a9_c58143e835f9>
        <rdfs:label xml:lang="en">solid</rdfs:label>
    </owl:Class>



    <!-- http://emmc.info/emmo-material#EMMO_db03061b_db31_4132_a47a_6a634846578b -->

    <owl:Class rdf:about="http://emmc.info/emmo-material#EMMO_db03061b_db31_4132_a47a_6a634846578b">
        <emmo-core:EMMO_967080e5_2f42_4eb2_a3a9_c58143e835f9>A standalone atom with an unbalanced number of electrons with respect to its atomic number.</emmo-core:EMMO_967080e5_2f42_4eb2_a3a9_c58143e835f9>
        <rdfs:comment>The ion_atom is the basic part of a pure ionic bonded compound i.e. without eclectron sharing,</rdfs:comment>
        <rdfs:label xml:lang="en">ion_atom</rdfs:label>
    </owl:Class>



    <!-- http://emmc.info/emmo-material#EMMO_df808271_df91_4f27_ba59_fa423c51896c -->

    <owl:Class rdf:about="http://emmc.info/emmo-material#EMMO_df808271_df91_4f27_ba59_fa423c51896c">
        <rdfs:subClassOf>
            <owl:Restriction>
                <owl:onProperty rdf:resource="http://emmc.info/emmo-direct#EMMO_b2282816_b7a3_44c6_b2cb_3feff1ceb7fe"/>
                <owl:someValuesFrom rdf:resource="http://emmc.info/emmo-material#EMMO_72d53756_7fb1_46ed_980f_83f47efbe105"/>
            </owl:Restriction>
        </rdfs:subClassOf>
        <rdfs:label xml:lang="en">neutron</rdfs:label>
    </owl:Class>



    <!-- http://emmc.info/emmo-material#EMMO_e5488299_8dab_4ebb_900a_26d2abed8396 -->

    <owl:Class rdf:about="http://emmc.info/emmo-material#EMMO_e5488299_8dab_4ebb_900a_26d2abed8396">
        <rdfs:subClassOf rdf:resource="http://emmc.info/emmo-core#EMMO_0f795e3e_c602_4577_9a43_d5a231aa1360"/>
        <owl:disjointUnionOf rdf:parseType="Collection">
            <rdf:Description rdf:about="http://emmc.info/emmo-material#EMMO_25f8b804_9a0b_4387_a3e7_b35bce5365ee"/>
            <rdf:Description rdf:about="http://emmc.info/emmo-material#EMMO_7db59e56_f68b_48b7_ae99_891c35ae5c3b"/>
            <rdf:Description rdf:about="http://emmc.info/emmo-material#EMMO_eb3c61f0_3983_4346_a0c6_e7f6b90a67a8"/>
        </owl:disjointUnionOf>
        <rdfs:label xml:lang="en">massless</rdfs:label>
    </owl:Class>



    <!-- http://emmc.info/emmo-material#EMMO_eb3c61f0_3983_4346_a0c6_e7f6b90a67a8 -->

    <owl:Class rdf:about="http://emmc.info/emmo-material#EMMO_eb3c61f0_3983_4346_a0c6_e7f6b90a67a8">
        <rdfs:label xml:lang="en">graviton</rdfs:label>
    </owl:Class>



    <!-- http://emmc.info/emmo-material#EMMO_eb77076b_a104_42ac_a065_798b2d2809ad -->

    <owl:Class rdf:about="http://emmc.info/emmo-material#EMMO_eb77076b_a104_42ac_a065_798b2d2809ad">
        <rdfs:subClassOf rdf:resource="http://emmc.info/emmo-material#EMMO_5c4aff3c_c30c_4507_86d5_b4df41eb9f2f"/>
        <rdfs:subClassOf>
            <owl:Restriction>
                <owl:onProperty rdf:resource="http://emmc.info/emmo-direct#EMMO_b2282816_b7a3_44c6_b2cb_3feff1ceb7fe"/>
                <owl:qualifiedCardinality rdf:datatype="http://www.w3.org/2001/XMLSchema#nonNegativeInteger">1</owl:qualifiedCardinality>
                <owl:onClass rdf:resource="http://emmc.info/emmo-material#EMMO_1067b97a_84f8_4d22_8ace_b842b8ce355c"/>
            </owl:Restriction>
        </rdfs:subClassOf>
        <rdfs:subClassOf>
            <owl:Restriction>
                <owl:onProperty rdf:resource="http://emmc.info/emmo-direct#EMMO_b2282816_b7a3_44c6_b2cb_3feff1ceb7fe"/>
                <owl:qualifiedCardinality rdf:datatype="http://www.w3.org/2001/XMLSchema#nonNegativeInteger">1</owl:qualifiedCardinality>
                <owl:onClass rdf:resource="http://emmc.info/emmo-material#EMMO_f835f4d4_c665_403d_ab25_dca5cc74be52"/>
            </owl:Restriction>
        </rdfs:subClassOf>
        <emmo-core:EMMO_967080e5_2f42_4eb2_a3a9_c58143e835f9>An &apos;atom&apos; is a &apos;nucleus&apos; surrounded by an &apos;electron_cloud&apos;, i.e. a quantum system made of one or more bounded electrons.</emmo-core:EMMO_967080e5_2f42_4eb2_a3a9_c58143e835f9>
        <emmo-core:EMMO_b432d2d5_25f4_4165_99c5_5935a7763c1a>A standalone atom has direct part one &apos;nucleus&apos; and one &apos;electron_cloud&apos;.

An O &apos;atom&apos; within an O2 &apos;molecule&apos; is an &apos;e-bonded_atom&apos;.

In this material branch, H atom is a particular case, with respect to higher atomic number atoms, since as soon as it shares its electron it has no nucleus entangled electron cloud.

We cannot say that H2 molecule has direct part two H atoms, but has direct part two H nucleus.</emmo-core:EMMO_b432d2d5_25f4_4165_99c5_5935a7763c1a>
        <rdfs:label xml:lang="en">atom</rdfs:label>
    </owl:Class>



    <!-- http://emmc.info/emmo-material#EMMO_f835f4d4_c665_403d_ab25_dca5cc74be52 -->

    <owl:Class rdf:about="http://emmc.info/emmo-material#EMMO_f835f4d4_c665_403d_ab25_dca5cc74be52">
        <rdfs:subClassOf rdf:resource="http://emmc.info/emmo-material#EMMO_7d66bde4_b68d_41cc_b5fc_6fd98c5e2ff0"/>
        <rdfs:subClassOf>
            <owl:Restriction>
                <owl:onProperty rdf:resource="http://emmc.info/emmo-direct#EMMO_b2282816_b7a3_44c6_b2cb_3feff1ceb7fe"/>
                <owl:someValuesFrom rdf:resource="http://emmc.info/emmo-material#EMMO_50781fd9_a9e4_46ad_b7be_4500371d188d"/>
            </owl:Restriction>
        </rdfs:subClassOf>
        <rdfs:subClassOf>
            <owl:Restriction>
                <owl:onProperty rdf:resource="http://emmc.info/emmo-direct#EMMO_b2282816_b7a3_44c6_b2cb_3feff1ceb7fe"/>
                <owl:minQualifiedCardinality rdf:datatype="http://www.w3.org/2001/XMLSchema#nonNegativeInteger">1</owl:minQualifiedCardinality>
                <owl:onClass rdf:resource="http://emmc.info/emmo-material#EMMO_8f87e700_99a8_4427_8ffb_e493de05c217"/>
            </owl:Restriction>
        </rdfs:subClassOf>
        <rdfs:label xml:lang="en">nucleus</rdfs:label>
    </owl:Class>



    <!--
    ///////////////////////////////////////////////////////////////////////////////////////
    //
    // Annotations
    //
    ///////////////////////////////////////////////////////////////////////////////////////
     -->

    <rdf:Description rdf:about="http://emmc.info/emmo-core#EMMO_04955fb5_4912_4729_8a19_35276e380b43">
        <rdfs:comment>“Granularity” stands for “matter with a particular granularity” .

Granularity is then defined as a superclass of defined subclasses that are defined as matter that is composed of specific types of objects
(and vacuum) and whose partitions respect direct parthood criteria.

The granularity class (and its inherited classes) is useful since a reasoner can automatically puts the individuals defined by the user under a generic class that expresses clearly the types of its compositional parts.

Since most of physics based modelling tools are designed to describe systems made of a specific base-object (e.g. atoms, fluids, particles) the granularity classes can be directly linked to model types.</rdfs:comment>
    </rdf:Description>
    <rdf:Description rdf:about="http://emmc.info/emmo-core#EMMO_13399199_cb46_4641_a951_cf032d5996ae">
        <emmo-core:EMMO_967080e5_2f42_4eb2_a3a9_c58143e835f9>A 1D (space) + 0D (time) substrate.</emmo-core:EMMO_967080e5_2f42_4eb2_a3a9_c58143e835f9>
    </rdf:Description>
    <rdf:Description rdf:about="http://emmc.info/emmo-core#EMMO_1703b6d9_b780_4c61_a75b_5f0cd39323e3">
        <rdfs:comment>A &apos;process&apos; individual is easily defined as a temporal part of a physical that is categorized in a primitive process subclass according to what type of process we want to represent.

Strictly speaking, every physical is a ‘process’ since it always has a time dimension, but here we restrict the meaning of ‘process’ to physicals whose evolution in time have a meaning for the material ontologist.

Participants of a process are always parts of that particular process (i.e. they are spacetime). It means that is_participant relation is subclass of is_part_of relation (e.g. you cannot participate to a party if you are not enclosed by the party room)</rdfs:comment>
    </rdf:Description>
    <rdf:Description rdf:about="http://emmc.info/emmo-core#EMMO_2d2ecd97_067f_4d0e_950c_d746b7700a31">
        <rdfs:comment>A &apos;set&apos; individual cannot be member of a &apos;set&apos; (to avoid Russel&apos;s paradox).</rdfs:comment>
        <emmo-core:EMMO_967080e5_2f42_4eb2_a3a9_c58143e835f9>The class representing the collection of all the individuals (signs) that represents a collection of &apos;item&apos; individuals.</emmo-core:EMMO_967080e5_2f42_4eb2_a3a9_c58143e835f9>
    </rdf:Description>
    <rdf:Description rdf:about="http://emmc.info/emmo-core#EMMO_2efbd83b_97c7_412a_805e_9866aa572885">
        <emmo-core:EMMO_967080e5_2f42_4eb2_a3a9_c58143e835f9>A 1D (space) + 1D (time) substrate.</emmo-core:EMMO_967080e5_2f42_4eb2_a3a9_c58143e835f9>
    </rdf:Description>
    <rdf:Description rdf:about="http://emmc.info/emmo-core#EMMO_3769c91c_b851_44c5_8fca_50751dd81d0a">
        <rdfs:comment>Matter is always 4D! There is no 3D representation of matter.

There can be a 3D slice of a matter but is no more matter: it’s simply a 3D spatial region.</rdfs:comment>
    </rdf:Description>
    <rdf:Description rdf:about="http://emmc.info/emmo-core#EMMO_54dc7f83_6c93_4bec_a0ff_3ea96f6ce16a">
        <emmo-core:EMMO_967080e5_2f42_4eb2_a3a9_c58143e835f9>A 2D (space) + 0D (time) substrate.</emmo-core:EMMO_967080e5_2f42_4eb2_a3a9_c58143e835f9>
    </rdf:Description>
    <rdf:Description rdf:about="http://emmc.info/emmo-core#EMMO_6a572193_effc_43a1_ab52_b2cec846b37e">
        <emmo-core:EMMO_967080e5_2f42_4eb2_a3a9_c58143e835f9>A 0D (space) + 0D (time) substrate.</emmo-core:EMMO_967080e5_2f42_4eb2_a3a9_c58143e835f9>
    </rdf:Description>
    <rdf:Description rdf:about="http://emmc.info/emmo-core#EMMO_7152d8e4_7c94_4a67_87b9_6de9c021e1b5">
        <emmo-core:EMMO_967080e5_2f42_4eb2_a3a9_c58143e835f9>A 3D (space) + 0D (time) substrate.</emmo-core:EMMO_967080e5_2f42_4eb2_a3a9_c58143e835f9>
    </rdf:Description>
    <rdf:Description rdf:about="http://emmc.info/emmo-core#EMMO_75bfd283_ff56_4a97_b05e_a3ea15d5e0a8">
        <emmo-core:EMMO_967080e5_2f42_4eb2_a3a9_c58143e835f9>A model is an abstraction for a physical entity.</emmo-core:EMMO_967080e5_2f42_4eb2_a3a9_c58143e835f9>
        <rdfs:comment>A model can be an abstraction for simple entities (e.g. an atom, a field) or a more complex existent.</rdfs:comment>
    </rdf:Description>
    <rdf:Description rdf:about="http://emmc.info/emmo-core#EMMO_a984ae65_ea32_44aa_9fab_c8493fe6d3e0">
        <emmo-core:EMMO_967080e5_2f42_4eb2_a3a9_c58143e835f9>A 2D (space) + 1D (time) substrate.</emmo-core:EMMO_967080e5_2f42_4eb2_a3a9_c58143e835f9>
    </rdf:Description>
    <rdf:Description rdf:about="http://emmc.info/emmo-core#EMMO_ac8e5770_cb05_4d82_ac83_93de968cdd8e">
        <emmo-core:EMMO_967080e5_2f42_4eb2_a3a9_c58143e835f9>A 0D (space) + 1D (time) substrate.</emmo-core:EMMO_967080e5_2f42_4eb2_a3a9_c58143e835f9>
    </rdf:Description>
    <rdf:Description rdf:about="http://emmc.info/emmo-core#EMMO_d82fd6c6_aebe_440f_9dd2_24a4eb3a417b">
        <emmo-core:EMMO_967080e5_2f42_4eb2_a3a9_c58143e835f9>A 3D (space) + 1D (time) substrate.</emmo-core:EMMO_967080e5_2f42_4eb2_a3a9_c58143e835f9>
        <rdfs:comment>The EMMO basic assumption is that the real world (the world outside us) manifests itself as a one spacetime entity, the Universe.

Some mereological parts (regions) of the Universe express peculiar properties that can be perceived by (they interact with) an interpreter/ontologist.

These mereological parts can be categorized in matter spacetimes or field spacetimes individuals.

&apos;physical&apos; class is the union of &apos;field&apos; and &apos;matter&apos; classes.</rdfs:comment>
    </rdf:Description>
    <rdf:Description rdf:about="http://emmc.info/emmo-core#EMMO_eb3a768e_d53e_4be9_a23b_0714833c36de">
        <rdfs:comment>The &apos;item&apos; class and all its sub-classes are &apos;set&apos; individuals.

The &apos;item&apos; branch will be used to represent the world things and can be seen in practice as the ontology core.</rdfs:comment>
        <emmo-core:EMMO_967080e5_2f42_4eb2_a3a9_c58143e835f9>The class that collects all the individuals that are member of a set (it’s the most comprehensive set individual).</emmo-core:EMMO_967080e5_2f42_4eb2_a3a9_c58143e835f9>
    </rdf:Description>
    <rdf:Description rdf:about="http://emmc.info/emmo-core#EMMO_eeb837b9_3995_4805_8662_5c2a59aeb494">
        <emmo-core:EMMO_967080e5_2f42_4eb2_a3a9_c58143e835f9>A 0D (space) + 0D (time) substrate.</emmo-core:EMMO_967080e5_2f42_4eb2_a3a9_c58143e835f9>
    </rdf:Description>
    <rdf:Description rdf:about="http://emmc.info/emmo-core#EMMO_f67528f5_7e45_405b_84e4_8a3b48aea914">
        <rdfs:comment>A &apos;substrate&apos; individual represents a place (in general sense) in which real world item exists.

A &apos;substrate&apos; individual provides the dimensions of existence for real world entities. It follows the fact that everything that exists is placed
somewhere and space and time coordinates can be used to identify
it.</rdfs:comment>
        <rdfs:comment>Substrate is the disjoint union of spacetime (4D), space (3D), surface (2D) and time (1D).</rdfs:comment>
        <rdfs:comment>This restriction in the mereological relations is done in order to overcome a typical misuse of the partitioning procedure, that occurs when the user wants to stretch the is_part_of relation beyond its applicability limit.

e.g. you can slice a 3D+1D cake in 3D+1D thin parts (3 spatial + 1 temporal dimension), but it’s impossible to slice the cake in infinitely thin 2D+1D slices (2 spatial + 1 temporal dimension). The relation of parthood applied to material entities cannot reduce spatial dimensions for a material object, since a 2D+1D material object does not exist!

Slicing a 3D+1D entity in a 2D+1D entity can still be done, but within the substrate level (the topological level) using
the is_slice_of relation working on geometrical concepts and not actual materials.</rdfs:comment>
    </rdf:Description>
    <rdf:Description rdf:about="http://emmc.info/emmo-core#EMMO_fee4fbb6_03a4_4e09_8af1_de772829963b">
        <emmo-core:EMMO_967080e5_2f42_4eb2_a3a9_c58143e835f9>A 0D (space) + 1D (time) substrate.</emmo-core:EMMO_967080e5_2f42_4eb2_a3a9_c58143e835f9>
    </rdf:Description>
</rdf:RDF>



<!-- Generated by the OWL API (version 4.5.7.2018-12-02T02:23:35Z) https://github.com/owlcs/owlapi -->
